Redo the increment device in Cava2. (#904)

firmware/IncrementWait/CavaIncrementDevice.v
@@ -1,113 +1,92 @@
-Require Import Cava.Cava.
-Import Circuit.Notations.
-Require Import Cava.CavaProperties.
 
+From Coq Require Import
+     Lists.List
+     ZArith.ZArith.
 
-Section WithCava.
-  Context {signal} {semantics : Cava signal}.
+Import ListNotations.
 
-  (* TODO doesn't Cava already provide these? *)
-  Definition ite{T: SignalType}(cond: signal Bit)(thn els: signal T):
-    cava (signal T) :=
-    branches <- packV (Vector.of_list [els; thn]);;
-    ctrl <- packV (Vector.of_list [cond]);;
-    indexAt branches ctrl.
+From Cava Require Import
+     Expr
+     Primitives
+     Semantics
+     Types
+     Util.BitArithmetic.
 
-  Definition and3: signal Bit * signal Bit * signal Bit -> cava (signal Bit) :=
-    fun '(x1, x2, x3) => x12 <- and2 (x1, x2);; and2 (x12, x3).
+Section Var.
+  Import ExprNotations.
+  Import PrimitiveNotations.
 
-  Definition or3: signal Bit * signal Bit * signal Bit -> cava (signal Bit) :=
-    fun '(x1, x2, x3) => x12 <- or2 (x1, x2);; or2 (x12, x3).
+  Context {var : tvar}.
 
-  Definition incr_update:
-    (* input: *)
-    signal Bit *             (* is_read_req *)
-    signal Bit *             (* is_write_req *)
-    signal (Vec Bit 32) *    (* req_addr (only relevant if is_reaq_req or is_write_req) *)
-    signal (Vec Bit 32) *    (* req_value (only relevant if is_write_req *)
-    (* state: *)
-    signal Bit *             (* idle *)
-    signal Bit *             (* busy *)
-    signal Bit *             (* done *)
-    signal (Vec Bit 32)      (* value *)
-    -> cava (
-    (* output: *)
-    signal Bit *             (* is_resp *)
-    signal (Vec Bit 32) *    (* resp (only relevant if is_resp *)
-    (* state: *)
-    signal Bit *             (* idle *)
-    signal Bit *             (* busy *)
-    signal Bit *             (* done *)
-    signal (Vec Bit 32))     (* value *)
-  := fun '(is_read_req, is_write_req, req_addr, req_value, idle, busy, done, value) =>
-       initialized <- or3 (idle, busy, done);;
-       idle <- ite initialized idle (constant true);;
-       is_resp <- or2 (is_read_req, is_write_req);;
-       (* bit #2 of the address determines if STATUS or VALUE register *)
-       req_addr1 <- Vec.tl req_addr;;
-       req_addr2 <- Vec.tl req_addr1;;
-       is_status_req <- Vec.hd req_addr2;;
-       is_value_req <- inv is_status_req;;
-       is_value_write_req <- and2 (is_value_req, is_write_req);;
-       isnt_value_write_req <- inv is_value_write_req;;
-       is_value_read_req <- and2 (is_value_req, is_read_req);;
-       no_pending_inp <- inv is_resp;;
-       result_ready <- or2 (busy, done);;
-       done2idle <- and2 (done, is_value_read_req);;
-       not_done2idle <- inv done2idle;;
-       idle2idle <- and2 (idle, isnt_value_write_req);;
-       idle' <- or2 (idle2idle, done2idle);;
-       busy' <- is_value_write_req;;
-       done' <- and2 (result_ready, not_done2idle);;
-       value_plus_one <- incrN value;;
-       value_or_input <- ite is_value_write_req req_value value;;
-       value' <- ite busy value_plus_one value_or_input;;
-       zeros <- Vec.const (constant false) 29;;
-       v1 <- Vec.cons done zeros;;
-       v2 <- Vec.cons busy v1;;
-       v3 <- Vec.cons idle v2;;
-       resp <- ite is_status_req v3 value;;
-       ret (is_resp, resp, idle', busy', done', value').
+  Local Open Scope N.
 
-  Definition incr: Circuit (signal Bit * signal Bit * signal (Vec Bit 32) * signal (Vec Bit 32))
-                           (signal Bit * signal (Vec Bit 32)) :=
-    Loop (Loop (Loop (Loop (Comb incr_update)))).
+  (* Things that should probably be in cava *)
+  Section Cava.
+    Definition state_of {i s o} (c : Circuit s i o) := denote_type s.
+  End Cava.
 
-End WithCava.
+  Definition incr
+    : Circuit _
+              (* Input *)
+              [ Bit          (* is_read_req *)
+                ; Bit        (* is_write_req *)
+                ; BitVec 32  (* req_addr (only relevant if is_read_req or is_write_req) *)
+                ; BitVec 32 ](* req_value (only relevant if is_write_req *)
+              (* Output *)
+              (Bit             (* is_resp *)
+                 ** BitVec 32) (* resp (only relevant if is_resp *)
+    := {{
+      fun is_read_req is_write_req req_addr req_value =>
+        (* bit #2 of the address determines if STATUS or VALUE register *)
+        let is_value_addr := (req_addr & (`K 1` << 2)) == `K 0` in
+        let is_value_write_req := is_value_addr && is_write_req in
+        let is_value_read_req := is_value_addr && is_read_req in
 
-Definition incr_device_step:
-  (* input: current state, is_read_req, is_write_req, req_addr, req_value *)
-  circuit_state incr -> bool * bool * Bvector 32 * Bvector 32 ->
-  (* output: next state, is_resp, resp *)
-  circuit_state incr * (bool * Bvector 32)
-  := step incr.
+        let/delay '(idle, busy, done; value) :=
+           if busy == `K 1` then
+             (`False`, `K 2`, `False`, value)
+           else if busy == `K 2` then
+                  (`False`, `K 0`, `True`, value + `K 1`)
+                else if done then
+                       (is_value_read_req, `K 0`, !is_value_read_req, value)
+                     else (* idle *)
+                       let busy' := if is_value_write_req then `K 1` else `K 0` in
+                       (!is_value_write_req, busy', `False`, req_value)
+           initially (false, (0, (false ,0))) : denote_type (Bit ** BitVec 2 ** Bit ** BitVec 32)
+        in
+
+        let status := if done then `K 1` else `K 0` in
+        let status := (status << 1) | (if busy == `K 0` then `K 0` else `K 1`) in
+        let status := (status << 1) | (if idle then `K 1` else `K 0`) in
+
+        let is_resp := is_read_req || is_write_req in
+        let resp := if is_value_addr then value else status in
+        (is_resp, resp)
+       }}.
+End Var.
+
+Example sample_trace :=
+  Eval compute in simulate incr
+                           [ (false,    (false, (111%N, (111%N, tt)))) (* no action *)
+                             ; (false,  (true,  (  0%N, ( 15%N, tt)))) (* write VALUE:=15 *)
+                             ; (true,   (false, (  4%N, (111%N, tt)))) (* read STATUS *)
+                             ; (true,   (false, (  4%N, (111%N, tt)))) (* read STATUS *)
+                             ; (true,   (false, (  0%N, (111%N, tt)))) (* read VALUE *)
+                           ].
+
+Definition incr_device_step s (input : bool * bool * N * N) : (_ * (bool * N)) :=
+  let '(is_read_req, is_write_req, req_addr, req_value) := input in
+  step incr s (is_read_req,
+               (is_write_req,
+                (req_addr, (req_value, tt)))).
 
 Require Import coqutil.Datatypes.List.
-
-(* like `simulate`, but also output the internal state, for more insightful debugging *)
-Fixpoint simulate_with_state_rec{i o}(c: Circuit i o)(initial: circuit_state c)(inps: list i)
-  : list (circuit_state c * o) :=
-  match inps with
-  | [] => []
-  | inp :: rest => let r := step c initial inp in r :: simulate_with_state_rec c (fst r) rest
-  end.
-Definition simulate_with_state{i o}(c: Circuit i o): list i -> list (circuit_state c * o) :=
-  simulate_with_state_rec c (reset_state c).
-
-Example sample_trace := Eval compute in simulate_with_state incr [
-  (false, false, N2Bv_sized 32 111, N2Bv_sized 32 111); (* no action *)
-  (false, true, N2Bv_sized 32 0, N2Bv_sized 32 15);     (* write VALUE:=15 *)
-  (true, false, N2Bv_sized 32 4, N2Bv_sized 32 111);    (* read STATUS *)
-  (true, false, N2Bv_sized 32 4, N2Bv_sized 32 111);    (* read STATUS *)
-  (true, false, N2Bv_sized 32 0, N2Bv_sized 32 111)     (* read VALUE *)
-].
-
-(* Print sample_trace. *)
 
 Require Import Coq.ZArith.ZArith. Open Scope Z_scope.
 Require Import riscv.Utility.Utility.
 Require Import coqutil.Map.Interface coqutil.Map.Properties.
 Require Import coqutil.Word.Interface coqutil.Word.Properties.
+Require Import coqutil.Tactics.Tactics.
 Require Import coqutil.Tactics.Simp.
 Require Import bedrock2.ZnWords.
 Require Import Bedrock2Experiments.RiscvMachineWithCavaDevice.InternalMMIOMachine.
@@ -116,16 +95,21 @@ Require Import Bedrock2Experiments.IncrementWait.IncrementWaitSemantics.
 Require Import Bedrock2Experiments.StateMachineSemantics.
 Require Import Bedrock2Experiments.RiscvMachineWithCavaDevice.MMIOToCava.
 
+Require Import Cava.Util.Identity.
+Require Import Cava.Util.Tactics.
+
 Section WithParameters.
+  Instance var : tvar := denote_type.
+
   Context {word: Interface.word 32} {word_ok: word.ok word}
           {Mem: map.map word byte} {Registers: map.map Z word}.
 
-  Definition mk_counter_state(idle busy done: bool)(val: Bvector 32): circuit_state incr :=
-    (tt, (tt, (tt, (tt, (tt, val), done), busy), idle)).
+  Definition mk_counter_state idle busy done (val : N) : state_of incr :=
+    (idle, (busy, (done, val))).
 
   Global Instance counter_device: device := {|
-    device.state := circuit_state incr;
-    device.is_ready_state s := exists val idle, s = mk_counter_state idle false false val;
+    device.state := state_of incr;
+    device.is_ready_state s := exists val idle, s = mk_counter_state idle 0 false val;
     device.run1 := incr_device_step;
     device.addr_range_start := INCR_BASE_ADDR;
     device.addr_range_pastend := INCR_END_ADDR;
@@ -137,28 +121,37 @@ Section WithParameters.
   {| ncycles_processing := 15%nat |}.
 
   Ltac destruct_state s :=
-    destruct s as ([] & (([] & (([] & (([] & ([] & ?val)) & ?done)) & ?busy)) & ?idle)).
+    destruct s as (?idle & ?busy & ?done & ?value).
 
-  Inductive counter_related: IncrementWaitSemantics.state -> circuit_state incr -> Prop :=
+  Inductive counter_related: IncrementWaitSemantics.state -> state_of incr -> Prop :=
   | IDLE_related: forall val idle,
       (* after reset, all three bools are false, and idle will be set to true *)
-      counter_related IDLE (mk_counter_state idle false false val)
-  | BUSY_related: forall val ncycles,
+      counter_related IDLE (mk_counter_state idle 0 false val)
+  | BUSY1_related: forall val ncycles,
+      (1 < ncycles)%nat ->
+      counter_related (BUSY val ncycles) (mk_counter_state false 1 false (word_to_N val))
+  | BUSY2_related: forall val ncycles,
       (0 < ncycles)%nat ->
-      counter_related (BUSY val ncycles) (mk_counter_state false true false (word_to_bv val))
+      counter_related (BUSY val ncycles) (mk_counter_state false 2 false (word_to_N val))
   (* the hardware is already done, but the software hasn't polled it yet to find out,
      so we have to relate a software-BUSY to a hardware-done: *)
   | BUSY_done_related: forall val ncycles,
       counter_related (BUSY val ncycles)
-                      (mk_counter_state false false true (word_to_bv (word.add (word.of_Z 1) val)))
+                      (mk_counter_state false 0 true (word_to_N (word.add (word.of_Z 1) val)))
   | DONE_related: forall val,
-      counter_related (DONE val) (mk_counter_state false false true (word_to_bv val)).
+      counter_related (DONE val) (mk_counter_state false 0 true (word_to_N val)).
 
-  Axiom TODO: False.
+  (* This should be in bedrock2.ZnWords. It is use by ZnWords, which is used in
+     the two following Lemmas. *)
+  Ltac better_lia ::= Zify.zify; Z.to_euclidean_division_equations; Lia.lia.
 
-  Axiom word_to_bv_inj: forall x y, word_to_bv x = word_to_bv y -> x = y.
+  Lemma incrN_word_to_bv: forall x,
+      ((N.add (word_to_N x) 1) mod 4294967296)%N = word_to_N (word.add (word.of_Z 1) x).
+  Proof. intros. unfold word_to_N. ZnWords. Qed.
 
-  Axiom incrN_word_to_bv: forall v, incrN (word_to_bv v) = word_to_bv (word.add (word.of_Z 1) v).
+  Lemma Z_word_N: forall x,
+      (0 <= x < 2 ^ 32) -> word_to_N (word.of_Z x) = Z.to_N x.
+  Proof. intros. unfold word_to_N. ZnWords. Qed.
 
   Set Printing Depth 100000.
 
@@ -177,29 +170,22 @@ Section WithParameters.
       simpl in *. destruct H as (val & idle & H). subst. eauto using IDLE_related.
     - (* nonMMIO_device_step_preserves_state_machine_state: *)
       simpl in sL1, sL2. destruct_state sL1. destruct_state sL2.
-      cbn [device.run1 counter_device incr_device_step step incr incr_update Loop snd
-           ret bind monad CombinationalSemantics Identity.Monad_ident constant] in H0.
-      eapply pair_equal_spec in H0. destruct H0 as [E1 E2].
-      subst.
-      eapply pair_equal_spec in E1. destruct E1 as [_ E1].
-      eapply pair_equal_spec in E1. destruct E1 as [E1 E2]. simpl in E2. subst.
-      eapply pair_equal_spec in E1. destruct E1 as [_ E1].
-      eapply pair_equal_spec in E1. destruct E1 as [E1 E2]. simpl in E2. subst.
-      eapply pair_equal_spec in E1. destruct E1 as [_ E1].
-      eapply pair_equal_spec in E1. destruct E1 as [E1 E2]. simpl in E2. subst.
-      eapply pair_equal_spec in E1. destruct E1 as [_ E1].
-      eapply pair_equal_spec in E1. destruct E1 as [_ E1]. simpl in E1. subst.
-      inversion H; subst.
+      cbn in H0. simp.
+      inversion H; subst; simp;
+        (* try rewrite N.land_0_r; *)
+        try rewrite Bool.andb_false_r;
+        cbn.
       + (* IDLE_related: *)
-        cbn. rewrite andb_false_r. destruct idle; cbn; simpl; eapply IDLE_related.
-      + (* BUSY_related: *)
-        rewrite andb_false_r. cbn -[incrN]. change (Pos.to_nat 1) with 1%nat.
-        cbn -[incrN]. rewrite incrN_word_to_bv.
-        eapply BUSY_done_related.
+        apply IDLE_related.
+      + (* BUSY1_related: *)
+        apply BUSY2_related. Lia.lia.
+      + (* BUSY2_related: *)
+        rewrite incrN_word_to_bv.
+        apply BUSY_done_related.
       + (* BUSY_done_related: *)
-        cbn. rewrite andb_false_r. cbn. assumption.
+        apply BUSY_done_related.
       + (* DONE_related: *)
-        cbn. rewrite andb_false_r. cbn. assumption.
+        apply DONE_related.
     - (* state_machine_read_to_device_read: *)
       (* simpler because device.maxRespDelay=1 *)
       unfold device.maxRespDelay, device.runUntilResp, device.state, device.run1, counter_device.
@@ -208,98 +194,111 @@ Section WithParameters.
       unfold read_step in *.
       destruct r.
       + (* r=VALUE *)
-        simp.
-        cbn. rewrite andb_false_r. simpl.
-        unfold word_to_bv. rewrite word.unsigned_of_Z_nowrap by (cbv; intuition discriminate).
-        simpl. do 3 eexists. ssplit; try reflexivity. eapply IDLE_related.
+        simp. cbn. rewrite Z_word_N; try Lia.lia; []. cbn.
+        unfold word_to_N.
+        (* rewrite word.unsigned_of_Z_nowrap by (cbv; intuition discriminate). *)
+        simpl. do 3 eexists. ssplit; try reflexivity.
+        eapply IDLE_related.
       + (* r=STATUS *)
         destruct sH.
         * (* sH=IDLE *)
           destruct Hp1. subst. inversion H0. subst.
-          cbn. rewrite andb_false_r. simpl. unfold status_value, STATUS_IDLE.
-          unfold word_to_bv.
-          rewrite word.unsigned_of_Z_nowrap by (cbv; intuition discriminate).
+          cbn. repeat (rewrite Z_word_N; try Lia.lia; []; cbn).
+          unfold status_value, STATUS_IDLE, word_to_N.
+          (* rewrite word.unsigned_of_Z_nowrap by (cbv; intuition discriminate). *)
           do 3 eexists. ssplit; try reflexivity. 2: eapply IDLE_related.
           rewrite word.unsigned_slu. 2: rewrite word.unsigned_of_Z. 2: reflexivity.
           rewrite !word.unsigned_of_Z. unfold word.wrap. cbn.
           destruct idle; reflexivity.
         * (* sH=BUSY *)
-          simp.
-          destruct Hp1 as [H | H].
+          simp. destruct Hp1 as [H | H].
           -- (* transition to DONE *)
              destruct H; subst.
              simpl (state_machine.reg_addr _).
-             unfold STATUS_ADDR, INCR_BASE_ADDR, word_to_bv, status_value, STATUS_DONE.
+             unfold STATUS_ADDR, INCR_BASE_ADDR, word_to_N, status_value, STATUS_DONE.
              rewrite !word.unsigned_of_Z. unfold word.wrap. simpl.
              inversion H0; subst.
-             ++ (* BUSY_related *)
-                (* the transition that was used to show that sH is not stuck was a transition
-                   from BUSY to DONE returning a done flag, but since the device is still
-                   in BUSY state, it will still return the busy flag in this transition,
-                   so the transition we use to simulate what happened in the device is a
-                   BUSY-to-DONE transition returning a busy flag instead of a done flag *)
+             ++ (* BUSY1_related *)
                 destruct max_cycles_until_done. 1: inversion H3. clear H3.
                 exists (word.of_Z 2). (* <- bit #1 (busy) is set, all others are 0 *)
                 do 2 eexists.
-                rewrite !word.unsigned_of_Z. unfold word.wrap. cbn -[incrN].
+                rewrite !word.unsigned_of_Z. unfold word.wrap. cbn.
                 ssplit; try reflexivity.
-                ** simpl. rewrite incrN_word_to_bv. eapply BUSY_done_related.
-                ** right. eexists; ssplit; try reflexivity. eapply word.unsigned_inj.
-                   rewrite word.unsigned_slu. 2: rewrite word.unsigned_of_Z. 2: reflexivity.
-                   rewrite !word.unsigned_of_Z. reflexivity.
-             ++ (* BUSY_done_related *)
-                exists (word.of_Z 4). (* <- bit #2 (done) is set, all others are 0 *)
+                ** eapply BUSY2_related.
+                   instantiate ( 1 := max_cycles_until_done ).
+                   inversion H0; subst.
+                   Lia.lia.
+                ** right. eexists; ssplit; try reflexivity; []. ZnWords.
+             ++ (* BUSY2_related *)
+                (* the transition that was used to show that sH is not stuck was *)
+                (* a transition from BUSY to DONE returning a done flag, but *)
+                (* since the device is still in BUSY state, it will still return *)
+                (* the busy flag in this transition, so the transition we use to *)
+                (* simulate what happened in the device is a BUSY-to-DONE *)
+                (* transition returning a busy flag instead of a done flag. *)
+               exists (word.of_Z 4). (* <- bit #2 (done) is set, all others are 0 *)
+                (* destruct max_cycles_until_done. 1: inversion H3. clear H3. *)
                 do 2 eexists.
-                rewrite !word.unsigned_of_Z. unfold word.wrap. cbn -[incrN].
-                ssplit; try reflexivity.
-                ** simpl. eapply DONE_related.
-                ** left. split. 2: reflexivity. eapply word.unsigned_inj.
-                   rewrite word.unsigned_slu. 2: rewrite word.unsigned_of_Z. 2: reflexivity.
-                   rewrite !word.unsigned_of_Z. reflexivity.
+                rewrite !word.unsigned_of_Z. unfold word.wrap. cbn.
+                ssplit; try reflexivity; [|].
+                ** rewrite incrN_word_to_bv.
+                   eapply DONE_related.
+                ** left. eexists; ssplit; try reflexivity; []. ZnWords.
+             ++ (* BUSY_done_related *)
+               exists (word.of_Z 4). (* <- bit #2 (done) is set, all others are 0 *)
+                do 2 eexists.
+                rewrite !word.unsigned_of_Z. unfold word.wrap. cbn.
+                ssplit; try reflexivity; [|].
+                ** eapply DONE_related.
+                ** left. split; try reflexivity; []. ZnWords.
           -- (* stay BUSY *)
              destruct H as (n & ? & ? & ?); subst.
              simpl (state_machine.reg_addr _).
-             unfold STATUS_ADDR, INCR_BASE_ADDR, word_to_bv, status_value, STATUS_BUSY.
+             unfold STATUS_ADDR, INCR_BASE_ADDR, word_to_N, status_value, STATUS_BUSY.
              rewrite !word.unsigned_of_Z. unfold word.wrap. simpl.
              inversion H0; subst.
-             ++ (* BUSY_related *)
+             ++ (* BUSY1_related *)
                 exists (word.of_Z 2). (* <- bit #1 (busy) is set, all others are 0 *)
                 do 2 eexists.
-                rewrite !word.unsigned_of_Z. unfold word.wrap. cbn -[incrN].
+                rewrite !word.unsigned_of_Z. unfold word.wrap. cbn.
                 ssplit; try reflexivity.
-                ** simpl. rewrite incrN_word_to_bv. eapply BUSY_done_related.
-                ** right. eexists; ssplit; try reflexivity. eapply word.unsigned_inj.
-                   rewrite word.unsigned_slu. 2: rewrite word.unsigned_of_Z. 2: reflexivity.
-                   rewrite !word.unsigned_of_Z. reflexivity.
-             ++ (* BUSY_done_related *)
-                (* the transition that was used to show that sH is not stuck was a transition
-                   from BUSY to BUSY returning a busy flag, but since the device already is
-                   in done state, it will return a done flag in this transition,
-                   so the transition we use to simulate what happened in the device is a
-                   BUSY-to-DONE transition returning a done flag instead of a
-                   BUSY-to-BUSY transition returning a busy flag. *)
+                ** eapply BUSY2_related. instantiate (1 := n).
+                   Lia.lia.
+                ** right. eexists; ssplit; try reflexivity; []. ZnWords.
+             ++ (* BUSY2_related *)
                 exists (word.of_Z 4). (* <- bit #2 (done) is set, all others are 0 *)
                 do 2 eexists.
-                rewrite !word.unsigned_of_Z. unfold word.wrap. cbn -[incrN].
+                rewrite !word.unsigned_of_Z. unfold word.wrap. cbn.
+                ssplit; try reflexivity; [|].
+                ** rewrite incrN_word_to_bv.
+                   eapply DONE_related.
+                ** left. eexists; ssplit; try reflexivity; []. ZnWords.
+             ++ (* BUSY_done_related *)
+                (* the transition that was used to show that sH is not stuck was *)
+                (* a transition from BUSY to BUSY returning a busy flag, but *)
+                (* since the device already is in done state, it will return a *)
+                (* done flag in this transition, so the transition we use to *)
+                (* simulate what happened in the device is a BUSY-to-DONE *)
+                (* transition returning a done flag instead of a BUSY-to-BUSY *)
+                (* transition returning a busy flag. *)
+                exists (word.of_Z 4). (* <- bit #2 (done) is set, all others are 0 *)
+                do 2 eexists.
+                rewrite !word.unsigned_of_Z. unfold word.wrap. cbn.
                 ssplit; try reflexivity.
                 ** simpl. eapply DONE_related.
-                ** left. split. 2: reflexivity. eapply word.unsigned_inj.
-                   rewrite word.unsigned_slu. 2: rewrite word.unsigned_of_Z. 2: reflexivity.
-                   rewrite !word.unsigned_of_Z. reflexivity.
+                ** left. split. 2: reflexivity. ZnWords.
         * (* sH=DONE *)
           destruct Hp1. subst. inversion H0. subst.
           simpl (state_machine.reg_addr _).
-          unfold STATUS_ADDR, INCR_BASE_ADDR, word_to_bv, status_value, STATUS_DONE.
+          unfold STATUS_ADDR, INCR_BASE_ADDR, word_to_N, status_value, STATUS_DONE.
           cbn.
-          rewrite !word.unsigned_of_Z. unfold word.wrap. cbn -[Vec.hd Vec.tl incrN].
+          rewrite !word.unsigned_of_Z. unfold word.wrap. cbn.
           exists (word.of_Z 4). (* <- bit #2 (done) is set, all others are 0 *)
           do 2 eexists.
           rewrite !word.unsigned_of_Z. unfold word.wrap. cbn.
           ssplit; try reflexivity.
           ** simpl. eapply DONE_related.
-          ** eapply word.unsigned_inj.
-             rewrite word.unsigned_slu. 2: rewrite word.unsigned_of_Z. 2: reflexivity.
-             rewrite !word.unsigned_of_Z. reflexivity.
+          ** ZnWords.
     - (* state_machine_write_to_device_write: *)
       destruct H as (sH' & ? & ?). subst.
       unfold write_step in H1.
@@ -307,10 +306,10 @@ Section WithParameters.
       destruct sH; try contradiction. subst.
       inversion H0. subst.
       cbn.
-      unfold word_to_bv.
+      unfold word_to_N.
       rewrite word.unsigned_of_Z_nowrap by (cbv; intuition discriminate).
       cbn.
-      eexists _, _, _. ssplit; try reflexivity. destruct idle; eapply BUSY_related; lia.
+      eexists _, _, _. ssplit; try reflexivity. destruct idle; eapply BUSY1_related; Lia.lia.
     - (* read_step_unique: *)
       cbn in *. unfold read_step in *. simp.
       destruct v; destruct r; try contradiction; simp; try reflexivity.
